### 3.1. **The Fundamental Theorem of Algebra** 
It states that any polynomial can be factored into linear polynomials , as long it is solvable. Example :
$$(x − a_{0})(x − a_{1})...(x − a_{n}) = 0$$
Define *p(x)* as sample polynomial, and *p(x)** is the multiplication of those cofactors *t(x)* 


$$h(x) = \frac{p(x)}{t(x)}$$
Let practice : 
Give :
$$ p(x)  = x^3 - 3x^2 + 2x $$$$t(x) = (x-1)(x-2) $$
Verifier samples a random value 23, calculates  $$t = t(23) = (23 − 1)(23 − 2) = 462$$and gives 23 to the prover 
Prover calculates $$h(x) = p(x) t(x) = x$$Evaluates $$ p = p(23) = 10626 $$$$h = h(23) = 23 $$and provides p, h to the verifier 
Verifier then checks that :  $$p = t · h: 10626 = 462 · 23$$which is true, and therefore the statement is proven
### 3.2. Modular Arithmetic 
### 3.3. Encrypted Polynomial
Let define E  : $$E(x) = g^{v} (mod(n)) $$
Example, We have :
$$ p(x) = x^{3} - 3x^{2} + 2{x}$$

In this case, we have 1, -3, 2 as coefficients so we can evaluate the encrypted polynomial as follows:
$$
\begin{aligned}
E(x^{3})^{1}E(x^{2})^{-3}E(x^{})^{2}=
\\(g^{x^{3}})^{1}(g^{x^{2}})^{-3}(g^{x^{}})^{2}=
\\g^{1x^{3}-3x^{x^2}g^{2x}}=
\\g^{x^{3}-3x^{2}+2x}
\end{aligned}
$$


