# Chapter 3

## 3.1. **The Fundamental Theorem of Algebra**

It states that any polynomial can be factored into linear polynomials as long as it is solvable. 

Example:
$$(x - a_{0})(x - a_{1})...(x - a_{n}) = 0$$

Define *p(x)* as a sample polynomial, and *p(x)* is the multiplication of those cofactors *t(x)*.

$$h(x) = \frac{p(x)}{t(x)}$$

In particular:
Given:
$$p(x)  = x^3 - 3x^2 + 2x$$

$$t(x) = (x-1)(x-2)$$

The Verifier samples a random value 23, calculates  $$t = t(23) = (23 - 1)(23 - 2) = 462$$ and gives 23 to the Prover.

The Prover calculates $h(x) = p(x)$, $t(x) = x$, evaluates $$p = p(23) = 10626$$ $$h = h(23) = 23$$ and provides p, h to the Verifier.

The Verifier then checks that:  $$p = t \cdot h: 10626 = 462 \cdot 23$$ 
This is true, and therefore the statement is proven.

## 3.2. Modular Arithmetic 

## 3.3. Encrypted Polynomial

Let's define *E* : $$E(x) = g^{v} \pmod{n}$$

For example, we have:
$$p(x) = x^{3} - 3x^{2} + 2x$$

In this case, with coefficients 1, -3, 2, the encrypted polynomial can be evaluated as follows:

$$
\begin{aligned}
E(x^{3})^{1}E(x^{2})^{-3}E(x)^{2}= \\
 (g^{x^{3}})^{1}(g^{x^{2}})^{-3}(g^{x})^{2}= \\
 g^{1x^{3}-3x^{x^2}g^{2x}}= \\
 g^{x^{3}-3x^{2}+2x} \\
\end{aligned}
$$

*Verifier*:

* Generate a random *s*
* Calculate $E(s^{i}) = g^{s^{i}}$: same as the example above
* Evaluate the *target polynomial* with *s*: *t(s)*
* Provide to the Prover: $E(s^{0}),E(s^{1}),E(s^{2}),...,E(s^{d})$

*Prover*:

* Calculates $h(x) = \frac{p(x)}{t(x)}$
* Evaluates: $E(p(s))$, $E(h(s))=g^{h(s)}$
* Provides $g^{p}$, $g^{h}$

*Verifier*:

* Check that $p=t(s) \cdot h$, meaning: 
  $g^{p} = (g^{h})^{t(s)}$

If the Prover claims to have a satisfactory polynomial using only 2 powers $s^{3}$ and $s^{1}$, it is not possible to verify in the current protocol.

## 3.4. Restricting a Polynomial

The main idea is to sample a random $\alpha$, and the provider needs to calculate $a^{,} = a^{\alpha} \pmod{n}$, then provide the tuple $(a,a^{,})$ using an elliptic curve. This ensures that the provider can't extract $\alpha$ from the tuple $(a,a^{,})$ through brute force.

We can also apply this construction with the simple one-coefficient polynomial $f(x)= c \cdot x$.

The Verifier can now check the equality:  $(a^{c})^{\alpha} = (\alpha^{,})^{c}$

In summary:

*Verifier*:

* Chooses 2 random *s*, $\alpha$ and provides evaluations for $x=s$ and $(g^{s},g^{\alpha \cdot s})$
* *Prover*: Applies the coefficient c:  $((g^{s})^c,(g^{\alpha \cdot s})^{c})=(g^{c \cdot s},g^{\alpha \cdot s \cdot c})$
* *Verifier*: Checks

In particular, for a degree $d$ polynomial: 
$$p(x) = x^{3} - 3x^{2} + 2x$$ 

*Verifier*:

* Provides encrypted: $g^{s^{0}},g^{s^{1}}, \cdots,g^{s^{d}}$ and their *shifts* $g^{\alpha s^{0}},g^{\alpha s^{1}}, \cdots,g^{\alpha s^{d}}$

*Prover*:

* Evaluates the encrypted polynomial with $s$: 
$$g^{p} = g^{p(s)} =(g^{s_{0}})^{c_{0}} \cdot (g^{s_{1}})^{c_{1}} \cdots (g^{s_{d}})^{c_{d}} = g^{c_{0}s^{0} +c_{1}s^{1}+ \cdots+c_{d}s^{d}  } =g^{s^{3}} \cdot g^{-3s^{2}} \cdot g^{2s}=g^{s^{3}-3s^{2}+2s}$$       
$$\Rightarrow g^{{p}'} = g^{\alpha (s^{3}-3s^{2}+2s)}$$ 
*Verifier* checks :
  $$(g^{p})^{\alpha}=g^{{p}'}$$ 
  $$\Rightarrow (g^{s^{3}-3s^{2}+2s})^{\alpha} = g^{\alpha (s^{3}-3s^{2}+2s)}$$ 

##### Conclusion

* We can be sure that the Prover did not use anything else other than the polynomial provided by the Verifier since there is no other way to preserve $\alpha$. 
* However, there is still a significant drawback: *The Verifier could **brute-force** a limited range of coefficient combinations until the result is **equal** to the Prover's answer*.
* Moreover, the secure protocol should be secure even in cases where there is only one coefficient, and its value is 1.

## 3.5. Zero-Knowledge 

Because the Verifier can extract knowledge about the unknown polynomial $p(x)$ only from the data sent by the Prover. So we can *shift* $g^{p}$, $(g^{p})^{\alpha}$ by a random number $\delta$.

## 3.6. Non-Interactivity 

Up to this point, the proof is only valid for the original Verifier because:

* The Verifier could collude with the Prover and disclose those secret parameters s, Î±.
* The Verifier has to store $\alpha$ and $t(s)$ until all relevant proofs are verified.

Hence, we need to

 secure the secrets $(t(s),\alpha)$, and this is where *cryptographic pairing* fits in.

### 3.6.1. Multiplication of Encrypted Values

Cryptographic pairings (bilinear map) have the core properties that can be expressed as:
$$e(g^{a},g^{b})=e(g^{b},g^{a})=e(g^{ab},g^{1})=e(g^{1},g^{ab})=e(g^{1},g^{a})^{b}=e(g^{1},g^{1})^{ab}= \cdots$$

### 3.6.2. Trusted Party Setup 

We trust a single party to generate secrets $s$ and $\alpha$. As soon as $\alpha$ and all necessary powers of $s$ with *shift* are encrypted, they must be deleted. So we use a *common reference string* or **CRS** to generate these parameters.

### 3.6.3. Trusting One out of Many 

There is no way to prove that $\alpha$ and s are deleted. So we can generate a composite CRS by multiple parties. 

In particular: 
* Alice samples her random $s_{A}$ and $\alpha_{A}$ and publishes her CRS:  $g^{s_{A}^{i}},g^{\alpha_{A}},g^{\alpha_{A}s_{A}^{i}}$  
* Bob samples his $s_{B}$ and $\alpha_{B}$ and  Alice's CRS through homomorphic multiplication: $(g^{s_{A}^{i}})^{s_{B}^{i}},(g^{\alpha_{A}})^{\alpha_{B}},(g^{\alpha_{A}s_{A}^{i}})^{\alpha_{B}s_{B}^{i}}$, then publishes A-B's CRS: $(g^{s_{AB}^{i}},g^{\alpha A B},g^{\alpha_{AB}s_{AB}^{i}})$ 
* So does with C, D, E, $\cdots$.

**Conclusion**: *The more there are unrelated participants in CRS setup, the fainter the possibility of fake proofs*

## 3.7.  Succinct Non-Interactive Argument of Knowledge of Polynomial

Denote ${s^{i}}_{i\in[d]} = s^{1},s^{2}, \cdots,s^{d}$

#### Setup 
- Sample random values $s,\alpha$
- Calculate $g^{\alpha}$ and $g^{s^{i}}$, $g^{\alpha s^{i}}$
- Proving key ($g^{s^{i}},g^{\alpha s^{i}}$)
- Verification key: ($g^{\alpha}$ ,$g^{t(s)}$)

#### Proving 
* Assign coefficients $(c_{i})_{i \in 0,...,d}$ :

$$p(x)= c_{d}x^{d} +\cdots+ c_{1}x^{1}+c_{0}x^{0}$$

* Calculate $h(x)= \frac{p(x)}{t(x)}$ 
* Evaluate $g^{p(s)}$ and $g^{h(s)}$ using $g^{s^{i}}$ 
* Evaluate $g^{\alpha p(s)}$ using $g^{\alpha s^{i}}$ 
* Sample random $\delta$ 
* Set the randomized proof $\pi = (g^{\delta p(s)}g^{\delta h(s)},g^{\delta \alpha p(s)})$

#### Verification 
Check:
* $e({g^{{p}'}},g)=e(g^{p},g^{\alpha})$ 
* $e(g^{p},g)=e(g^{t(s)},g^{h})$